Upd

SkipList2/SkipList2.Properties.fst
@@ -4,24 +4,28 @@ open FStar.Seq
 open FStar.Option
 open SkipList2.Statement
 module List = FStar.List.Tot
+module Sl = SkipList2.Statement
 
 type cmp (a:eqtype) = f:(a -> a -> Tot bool){total_order a f}
 
-(*)
-assume val lemma_index_1 : #a: eqtype -> #f:(cmp a) -> sl: skipList a f -> 
-	Lemma(ensures 
-		(forall (counter:nat{counter<(length sl)}). List.for_all (fun (x:nat) -> x < length sl) (getIndex sl counter)))
-*)
 
-assume val lemma_index_1: #a: eqtype -> #f: (cmp a) -> sl: skipList a f  -> 
+assume val lemma_last_element_biggest: #a : eqtype -> #f: cmp(a)  ->  sl: skipList a f{Sl.length sl > 1} -> value: a
+-> Lemma (ensures (f value (last_element_values  #a #f sl)))	
+
+assume val lemma_index_3 : #a: eqtype -> #f: cmp a -> sl:skipList a f {Sl.length sl > 1} -> 
+					counter_global:nat{counter_global < (Sl.length sl -1)} -> 
+					Lemma(ensures(last_element_indexed #a #f sl counter_global = counter_global +1))
+
+
+assume val lemma_index_1: #a: eqtype -> #f: (cmp a) -> sl: skipList a f{length sl> 1}  -> 
 	Lemma(ensures
 		(forall (counter_global: nat {counter_global < length sl}) 
 		(counter_local : nat 
 			{counter_local <List.length
 				(getIndex sl counter_global)}). 
-		(fun (x: nat) -> x < length sl) (List.index(getIndex sl counter_global) counter_local)))
+		(fun (x: nat) -> x < (length sl)) (List.index(getIndex sl counter_global) counter_local)))
 
-assume val lemma_index_2: #a: eqtype -> #f: (cmp a) -> sl: skipList a f  -> 
+assume val lemma_index_2: #a: eqtype -> #f: (cmp a) -> sl: skipList a f {length sl> 1} -> 
 	Lemma(ensures
 		(forall (counter_global: nat {counter_global < length sl}) 
 		(counter_local : nat 
@@ -29,12 +33,31 @@ assume val lemma_index_2: #a: eqtype -> #f: (cmp a) -> sl: skipList a f  ->
 				(getIndex sl counter_global)}). 
 		(fun (x: nat) -> x > counter_global) (List.index(getIndex sl counter_global) counter_local)))
 
-assume val lemma_index_3 : #a : eqtype -> #f:(cmp a) -> sl: skipList a f ->
-	Lemma(ensures
-		(forall (counter : nat {counter < (length sl - 1)}).
-				List.index (getIndex sl counter) (List.length (getIndex sl counter) -1 ) = (counter + 1)
-		)
-	)
+val lemma_index_1_wrapper: #a: eqtype -> #f: (cmp a) -> sl: skipList a f{Sl.length sl> 1} -> 
+		counter_global: nat{counter_global < Sl.length sl} -> 
+		counter_local : nat{ counter_local <List.length
+				(getIndex sl counter_global)} -> Tot(r: nat{ r< (Sl.length sl)} )
+let lemma_index_1_wrapper #a #f sl counter_global counter_local = 
+	let i = getIndex sl counter_global in 
+	let l = List.index i counter_local in
+	lemma_index_1 #a #f sl; l
+val lemma_index_2_wrapper: #a: eqtype -> #f: (cmp a) -> sl: skipList a f{Sl.length sl> 1} -> 
+		counter_global: nat{counter_global < Sl.length sl} -> 
+		counter_local : nat{ counter_local <List.length
+				(getIndex sl counter_global)} -> Tot(r: nat{ r > counter_global} )
+let lemma_index_2_wrapper #a #f sl counter_global counter_local = 
+	let i = getIndex sl counter_global in 
+	let l = List.index i counter_local in
+	lemma_index_2 #a #f sl; l
+val lemma_index_1_2_wrapper: #a: eqtype -> #f: (cmp a) -> sl: skipList a f{Sl.length sl> 1} -> 
+		counter_global: nat{counter_global < Sl.length sl} -> 
+		counter_local : nat{ counter_local <List.length
+				(getIndex sl counter_global)} -> Tot(r: nat{ r > counter_global /\ r< (Sl.length sl)} )
+let lemma_index_1_2_wrapper #a #f sl counter_global counter_local = 
+	let i = getIndex sl counter_global in 
+	let l = List.index i counter_local in
+	lemma_index_1 #a #f sl; lemma_index_2 #a #f sl; l	
+
 (*)
 val equal_whole_slice: #a: eqtype -> #f:(cmp a) ->
 			s:seq a {sorted f s} -> 
@@ -43,6 +66,9 @@ let equal_whole_slice #a #f s = ()
 
 val lemma_tail_size: s: seq 'a{length s > 0} -> Lemma (ensures (Seq.length s - 1 = (Seq.length (Seq.tail s ))))
 let lemma_tail_size s = ()			
+
+
+
 
 val lemma_sorted_tail : #a: eqtype -> #f:(cmp a) ->
 			s:seq a {sorted f s && length s > 0} -> 
@@ -56,12 +82,16 @@ val lemma_tail_slice : #a: eqtype -> #f:(cmp a) ->
 			))	
 let lemma_tail_slice #a #f s= ()
 
+
+
 val lemma_one_step_slice: #a : eqtype -> #f:(cmp a) -> 
 			s: seq a {sorted f s  && Seq.length s > 0} ->
 			Lemma (ensures
 				(equal (Seq.slice s 1 (Seq.length s)) (Seq.tail(Seq.slice s 0 (Seq.length s))))
 			)
 let lemma_one_step_slice #a #f s = ()
+
+
 
 (*slice j<=length s*)
 val lemma_one_step_slice_gen: #a: eqtype -> #f:(cmp a) -> 
